soundness proofs

LcfInLean/Basic.lean
@@ -13,11 +13,27 @@ inductive Term where
 | Impl (l : Term) (r : Term)
 deriving BEq, DecidableEq, Repr
 
+#check @Term.rec
+
 structure Theorem where
   -- NOTE: the head of this list is the last element of the hypotheses
   hypotheses : List Term
   conclusion : Term
 deriving Repr
+
+-- map LCF terms into lean props.
+def mapTerm (assign : String → Prop) : (t : Term) → Prop
+| .Var s => assign s
+| .True => True
+| .False => False
+| .And l r => (mapTerm assign l) ∧ (mapTerm assign r)
+| .Or l r => (mapTerm assign l) ∨ (mapTerm assign r)
+| .Neg t => ¬ (mapTerm assign t)
+| .Impl l r => (mapTerm assign l) → (mapTerm assign r)
+
+-- construct the lean prop that asserts the validity of the input theorem
+def valid (t : Theorem) : Prop :=
+  ∀ (a : String → Prop), (∀ (p : Prop), p ∈ List.map (mapTerm a) t.hypotheses → p) → mapTerm a t.conclusion
 
 -- Utils --
 
@@ -45,14 +61,76 @@ def subst (nm : String) (t : Term) : (target : Term) → Term
 def and_intro (l : Theorem) (r : Theorem) : Theorem :=
   ⟨l.hypotheses ++ r.hypotheses, .And l.conclusion r.conclusion⟩
 
+theorem and_intro_sound (l r : Theorem) (hl : valid l) (hr : valid r) : valid (and_intro l r) := by
+  unfold and_intro
+
+  unfold valid at *
+  intro assign
+  intro hyp_valid
+  simp at *
+  unfold mapTerm
+
+  have hyp_l : ∀ (p : Prop), (∃ a ∈ l.hypotheses, mapTerm assign a ↔ p) → p := by
+    clear hl hr
+    intro p
+    specialize hyp_valid p
+    aesop
+  have hyp_r : ∀ (p : Prop), (∃ a ∈ r.hypotheses, mapTerm assign a ↔ p) → p := by
+    clear hl hr hyp_l
+    intro p
+    specialize hyp_valid p
+    aesop
+
+  have hl' : (∀ (p : Prop), ∀ x ∈ l.hypotheses, (mapTerm assign x ↔ p) → p) := by
+    clear hl hr hyp_valid hyp_r
+    aesop
+  have hr' : (∀ (p : Prop), ∀ x ∈ r.hypotheses, (mapTerm assign x ↔ p) → p) := by
+    clear hl hr hyp_valid hyp_l
+    aesop
+
+  clear hyp_valid
+  specialize hl assign hl'
+  specialize hr assign hr'
+  clear hyp_l hyp_r hl' hr'
+  simp [*]
+
 def or_intro_l (l : Theorem) (t : Term) : Theorem :=
   ⟨l.hypotheses, Term.Or l.conclusion t⟩
+
+theorem or_intro_l_valid (l : Theorem) (t : Term) (hl : valid l) : valid (or_intro_l l t) := by
+  unfold valid at *
+  unfold or_intro_l
+  intros assign hyp_valid
+  simp at *
+  specialize hl assign
+  unfold mapTerm
+  apply Or.intro_left
+  specialize hl hyp_valid
+  assumption
 
 def or_intro_r (r : Theorem) (t : Term) : Theorem :=
   ⟨r.hypotheses, Term.Or t r.conclusion⟩
 
+theorem or_intro_r_valid (r : Theorem) (t : Term) (hr : valid r) : valid (or_intro_r r t) := by
+  unfold valid at *
+  unfold or_intro_r
+  intros assign hyp_valid
+  simp at *
+  specialize hr assign
+  unfold mapTerm
+  apply Or.intro_right
+  specialize hr hyp_valid
+  assumption
+
 def true : Theorem := ⟨[], Term.True⟩
+
+theorem true_valid : valid true := by simp [valid, true, mapTerm]
+
 def assume (t : Term) : Theorem := ⟨[t], t⟩
+
+theorem assume_valid (t : Term) : valid (LCF.assume t) := by
+  simp [valid, LCF.assume, mapTerm]
+  aesop
 
 def discharge (a : Term) (thm : Theorem) : Theorem :=
   ⟨List.filter (λ h => h != a) thm.hypotheses
@@ -93,6 +171,105 @@ def instantiate (var : String) (t : Term) (thm : Theorem) : Option Theorem :=
   then none
   else pure ⟨thm.hypotheses, subst var t thm.conclusion⟩
 
+theorem subst_preserves_validity (var : String) (t : Term) (hyps : List Term) (conclusion : Term) (ht : valid ⟨hyps, conclusion⟩) : valid ⟨List.map (subst var t) hyps, subst var t conclusion⟩ := by
+  unfold valid at *
+  intro assign
+  let assign' := λ var' => if var = var' then mapTerm assign t else assign var'
+  specialize ht assign'
+  have mapTermPres : ∀ (t' : Term), mapTerm assign' t' = mapTerm assign (subst var t t') := by
+    intro t'
+    induction t' with
+    | Var s =>
+      dsimp [assign']
+      rw (config := {occs := .pos [1]}) [mapTerm]
+      simp_all
+      split
+      case Var.isTrue h =>
+        unfold subst
+        simp_all
+      case Var.isFalse h =>
+        unfold subst
+        have nes : ¬ (s = var) := by aesop
+        simp_all
+        unfold mapTerm
+        rfl
+    | True => aesop
+    | False => aesop
+    | And l r hl hr => unfold mapTerm subst; simp_all
+    | Or l r hl hr => unfold mapTerm subst; simp_all
+    | Neg t ih => unfold mapTerm subst; simp_all
+    | Impl l r hl hr => unfold mapTerm subst; simp_all
+
+  induction hyps with
+  | nil => aesop
+  | cons hd tl ih_hyp =>
+    simp [*] at *
+    exact ht
+
+theorem instantiate_valid (var : String) (t : Term) (thm : Theorem) (ht : valid thm)
+  : match instantiate var t thm with
+    | .none => True
+    | .some res => valid res
+  := by
+    unfold instantiate
+    split
+    case h_1 => trivial
+    case h_2 x res heq =>
+      simp_all
+      unfold valid
+      have x_not_free : ¬ (∃ x ∈ thm.hypotheses, occurs_free var x = Bool.true) := by aesop
+      have res_eq : res = { hypotheses := thm.hypotheses, conclusion := subst var t thm.conclusion } := by aesop
+      clear heq
+      intros assign hyp_valid
+      rw [res_eq] at hyp_valid ⊢
+      simp [*] at hyp_valid ⊢
+      have subst_valid : valid ⟨List.map (subst var t) thm.hypotheses, subst var t thm.conclusion⟩ := subst_preserves_validity var t thm.hypotheses thm.conclusion ht
+      unfold valid at subst_valid
+      simp at subst_valid
+      specialize subst_valid assign
+      refine subst_valid ?h
+      intro p x hx
+      have not_free : ¬ (occurs_free var x) := by aesop
+      have subst_noop : subst var t x = x := by
+        clear hx
+        induction x with
+        | Var s' =>
+          unfold occurs_free at not_free
+          simp [subst]
+          aesop
+        | True => trivial
+        | False => trivial
+        | And l r hl hr =>
+          unfold subst
+          simp
+          apply And.intro
+          · unfold occurs_free at not_free
+            aesop
+          · unfold occurs_free at not_free
+            aesop
+        | Or l r hl hr =>
+          unfold subst
+          simp
+          apply And.intro
+          · unfold occurs_free at not_free
+            aesop
+          · unfold occurs_free at not_free
+            aesop
+        | Neg t' ht' =>
+          unfold subst
+          simp
+          unfold occurs_free at not_free
+          aesop
+        | Impl l r hl hr =>
+          unfold subst
+          simp
+          apply And.intro
+          · unfold occurs_free at not_free
+            aesop
+          · unfold occurs_free at not_free
+            aesop
+      aesop
+
 -- Structural --
 
 -- This applies all structural rules at once
@@ -100,6 +277,41 @@ def structural (thm : Theorem) (reordered : List Term) : Option Theorem :=
   if List.toFinset thm.hypotheses ⊆ List.toFinset reordered
   then pure ⟨reordered, thm.conclusion⟩
   else none
+
+theorem structural_valid (t : Theorem) (reord : List Term) (ht : valid t) :
+  match structural t reord with
+    | .none => True
+    | .some res => valid res
+  := by
+    unfold structural
+    split
+    case h_1 => trivial
+    case h_2 x res heq =>
+      simp_all
+      unfold valid
+      intros assign hyp_valid
+      rcases heq with ⟨hl, hr⟩
+      symm at hr
+      rw [hr]
+      rw [hr] at hyp_valid
+      simp_all
+      have valid_hyps : ∀ (p : Prop), ∀ x ∈ t.hypotheses, (mapTerm assign x ↔ p) → p := by
+        intros p x hx
+        specialize hyp_valid p
+        have : x ∈ reord := by
+          clear hr hyp_valid
+          have : x ∈ t.hypotheses → x ∈ t.hypotheses.toFinset := by aesop
+          have : x ∈ t.hypotheses.toFinset → x ∈ reord.toFinset := by
+            unfold Finset.instHasSubset at hl
+            aesop
+          aesop
+        aesop
+      unfold valid at ht
+      specialize ht assign
+      have valid_hyps' : (∀ p ∈ List.map (mapTerm assign) t.hypotheses, p) := by
+        clear hyp_valid hl hr ht
+        aesop
+      exact ht valid_hyps'
 
 -- the following are meta proofs that the above covers all structural rules,
 -- carried out by implementing the individual rules in terms of the above
